reorging DHE formats

src/tls/CommonDH.fst
@@ -68,6 +68,21 @@ let serialize k =
   | FFKey k -> DHGroup.serialize k.dh_params k.dh_public
   | ECKey k -> ECGroup.serialize k.ec_params k.ec_point
 
+val parse_partial: bytes -> bool -> Tot (TLSError.result (key * bytes)) 
+let parse_partial p ec = 
+    if ec then 	 
+      (match ECGroup.parse_partial p with
+       | Correct(eck,rem) -> 
+	 Correct (ECKey eck, rem)
+       | Error z -> Error z)
+    else 
+      (match DHGroup.parse_partial p with
+       | Correct(dhk,rem) -> 	   
+         Correct (FFKey dhk, rem)
+       | Error z -> Error z)
+
+        
+  
 // Serialize for keyShare extension
 val serialize_raw: key -> Tot bytes
 let serialize_raw = function
