src/tls/DHGroup.fst
@@ -101,3 +101,30 @@ let serialize_public dh_Y =
   lemma_repr_bytes_values (length dh_Y);
   vlbytes 2 dh_Y
 
+val parse_public: bytes -> Tot (result share)
+let parse_public p = 
+  vlparse 2 p
+
+val parse_partial: bytes -> Tot (result (key * bytes))
+let parse_partial payload = 
+    if length payload >= 2 then
+      match vlsplit 2 payload with
+      | Error(z) -> Error(z)
+      | Correct(res) ->
+        let (p,payload) = res in
+        if length payload >= 2 then
+          match vlsplit 2 payload with
+          | Error(z) -> Error(z)
+          | Correct(res) ->
+            let (g,payload) = res in
+            if length payload >= 2 then
+              match vlsplit 2 payload with
+              | Error(z) -> Error(z)
+              | Correct(res) ->
+	        let (gy,rem) = res in 
+		let dhp = {dh_p = p; dh_g = g; dh_q = None; safe_prime = false} in
+		let dhk = {dh_params = dhp; dh_public = gy; dh_private = None} in
+		Correct (dhk,rem)
+            else Error(AD_decode_error, perror __SOURCE_FILE__ __LINE__ "")
+        else Error(AD_decode_error, perror __SOURCE_FILE__ __LINE__ "")
+    else Error(AD_decode_error, perror __SOURCE_FILE__ __LINE__ "")
